
	با رسم درخت برهان ثابت کنید.
	$$
		\forall x \neg(p(x) \wedge q(x)) \vdash \forall x (\neg p(x) \vee \neg q(x))
	$$
	\newline
	\quad\vspace {0.5cm}
	\begin{ans}
		لم ۱ : 
		$$
			\neg (\forall x p(x)) \vdash \exists x \neg p(x)
		$$
		\newline
		$$
			\infer[RAA_1]{\exists x \neg p(x)}{
				\infer[\neg E]{\bot}{
					\infer[\forall I]{\forall x p(x)}{
						\infer[RAA_2]{p(x)}{
							\infer[\neg E]{\bot}{
								\infer[\exists I]{\exists x \neg p(x)}{
									[\neg p(x)]_2
								}
								&
								[\neg \exists x(\neg p(x))]_1
							}
						}	
					}
					&
					\neg(\forall x p(x))
				}
			}
		$$
		\pagebreak
		
		لم ۲ : 
		$$
			\neg(A \wedge B) \vdash (\neg A \vee \neg B)
		$$
		\newline
		$$
			\infer[RAA_1]{\neg A \vee \neg B}{
				\infer[\neg E]{\bot}{
					\infer[\wedge I]{A \wedge B}{
						\infer[RAA_2]{A}{
							\infer[\neg E]{\bot}{
								\infer[\vee I]{\neg A \vee \neg B}{
									[\neg A]_2
								}
								&
								[\neg(\neg A \vee \neg B)]_1
							}
						}
						&
						\infer[RAA_3]{B}{
							\infer[\neg E]{\bot}{
								\infer[\vee I]{\neg A \vee \neg B}{
									[\neg B]_3
								}
								&
								[\neg(\neg A \vee \neg B)]_1
							}
						}
					}
					&
					\neg (A \wedge B)
				}
			}
		$$
		
		$$
			\infer[RAA_1]{\forall x (\neg p(x) \vee \neg q(x))}{
				\infer[\exists E_2]{\bot}{
					\infer[\text{لم ۱}]{\exists x (\neg(\neg p(x) \vee \neg q(x)))}{
						[\neg(\forall x (\neg p(x) \vee \neg q(x)))]_1
					}
					&
					\infer[\neg E]{\bot}{
						[\neg (\neg p(c) \vee \neg q(c))]_2
						&
						\infer[\text{لم ۲}]{\neg p(c) \vee \neg q(c)}{
							\infer[\forall E]{\neg (p(x) \wedge q(x))}{
								\forall x \neg(p(x) \wedge q(x))
							}
						}
					}
				}
			}
		$$
		
	\end{ans}
	
