ثابت کنید:
\begin{enumerate}[label=(\alph*)]
    \item $\varphi\to(\psi\to\sigma)\dashv\vdash((\varphi\wedge\psi)\to\sigma)$
    \item $\vdash\neg(\varphi\to\psi)\to\neg\psi$
    \item $\varphi\to\psi\dashv\vdash\neg\psi\to\neg\varphi$
    \item $\vdash(\varphi\to\psi)\to(\neg\varphi\vee\psi)$
    \item $\varphi\vee\psi,\neg\varphi\vdash\psi$
    \item $\varphi\vee\psi\vdash\psi\vee\varphi$
\end{enumerate}\quad\vspace*{-0.5cm}
\begin{ans}
    \begin{enumerate}[label=(\alph*)]
        \item\quad\\\LTR
        \begin{prooftree}
            \AxiomC{$[\varphi\vee\psi]^1$}
            \conE{$\psi$}

            \AxiomC{$[\varphi\vee\psi]^1$}
            \conE{$\varphi$}
            \AxiomC{$\phi\to(\psi\to\sigma)$}
            \toE{$\phi\to\sigma$}

            \toE{$\sigma$}
            \toI[1]{$(\phi\wedge\psi)\to\sigma$}
        \end{prooftree}
        \begin{prooftree}
            \AxiomC{$[\phi]^2$}
            \AxiomC{$[\psi]^1$}
            \conI{$\phi\wedge\psi$}

            \AxiomC{$(\phi\wedge\psi)\to\sigma$}
            \toE{$\sigma$}
            \toI[1]{$\psi\to\sigma$}
            \toI[2]{$\phi\to(\psi\to\sigma)$}
        \end{prooftree}\RTL
        \item\quad\\
        \LTR\begin{prooftree}
            \AxiomC{$[\psi]^1$}
            \toI{$\phi\to\psi$}
            
            \AxiomC{$[\neg(\phi\to\psi)]^2$}
            \botI
            \negI[1]{$\neg\phi$}
            \toI[2]{$\neg(\phi\to\psi)\to\neg\phi$}
        \end{prooftree}\RTL
        \item\quad\\\LTR
        \begin{prooftree}
            \AxiomC{$[\varphi]^1$}
            \AxiomC{$\varphi\to\psi$}
            \toE{$\psi$}
            \AxiomC{$[\neg\psi]^2$}
            \botI
            \negI[1]{$\neg\varphi$}
            \toI[2]{$\neg\psi\to\neg\varphi$}
        \end{prooftree}
        \begin{prooftree}
            \AxiomC{$[\varphi]^2$}

            \AxiomC{$[\neg\psi]^1$}
            \AxiomC{$\neg\psi\to\neg\varphi$}
            \toE{$\neg\varphi$}

            \botI
            \RAA[1]{$\psi$}
            \toI[2]{$\varphi\to\psi$}
        \end{prooftree}\RTL
        \item\quad\\\LTR
        \begin{prooftree}
            \AxiomC{$[\varphi]^2$}
            \AxiomC{$[\varphi\to\psi]^4$}
            \toE{$\psi$}

            \AxiomC{$[\psi]^1$}
            \veeI{$\neg\varphi\vee\psi$}
            \AxiomC{$[\neg(\neg\varphi\vee\psi)]^3$}
            \botI
            \negI[1]{$\neg\psi$}

            \botI
            \RAA[3]{$\neg\varphi\vee\psi$}
            \toI[4]{$(\varphi\to\psi)\to(\neg\varphi\vee\psi)$}
        \end{prooftree}\RTL
        \item\quad\\\LTR
        \begin{prooftree}
            \AxiomC{$\varphi\vee\psi$}

            \AxiomC{$[\varphi]^1$}
            \AxiomC{$\neg\varphi$}
            \botI
            \botE{$\psi$}

            \AxiomC{$[\psi]^1$}

            \veeE{1}{$\psi$}
        \end{prooftree}\RTL
        \item\quad\\\LTR
        \begin{prooftree}
            \AxiomC{$\varphi\vee\psi$}

            \AxiomC{$[\varphi]^1$}
            \veeI{$\psi\vee\varphi$}

            \AxiomC{$[\psi]^1$}
            \veeI{$\psi\vee\varphi$}

            \veeE{1}{$\psi\vee\varphi$}
        \end{prooftree}
    \end{enumerate}

\end{ans}